q

softwarefoundations/vol2_plf/Equiv.v
@@ -255,3 +255,429 @@ Proof.
     constructor.
 Qed.
 
+
+
+Lemma refl_aequiv : forall (a : aexp), aequiv a a.
+Proof. intros a st. reflexivity. Qed.
+
+Lemma sym_aequiv : forall (a1 a2 : aexp), aequiv a1 a2 -> aequiv a2 a1.
+Proof. intros a1 a2 H. intros st. symmetry. apply H. Qed.
+
+Lemma trans_aequiv : forall (a1 a2 a3 : aexp), aequiv a1 a2 -> aequiv a2 a3 -> aequiv a1 a3.
+Proof.
+  unfold aequiv. intros a1 a2 a3 H12 H23 st.
+  rewrite (H12 st). rewrite (H23 st). reflexivity. Qed.
+
+Lemma refl_bequiv : forall (b : bexp), bequiv b b.
+Proof. unfold bequiv. intros b st. reflexivity. Qed.
+
+Lemma sym_bequiv : forall (b1 b2 : bexp), bequiv b1 b2 -> bequiv b2 b1.
+Proof. unfold bequiv. intros b1 b2 H. intros st. symmetry. apply H. Qed.
+
+Lemma trans_bequiv : forall (b1 b2 b3 : bexp), bequiv b1 b2 -> bequiv b2 b3 -> bequiv b1 b3.
+Proof.
+  unfold bequiv. intros b1 b2 b3 H12 H23 st.
+  rewrite (H12 st). rewrite (H23 st). reflexivity. Qed.
+
+Lemma refl_cequiv : forall (c : com), cequiv c c.
+Proof. unfold cequiv. intros c st st'. reflexivity. Qed.
+
+Lemma sym_cequiv : forall (c1 c2 : com), cequiv c1 c2 -> cequiv c2 c1.
+Proof.
+  unfold cequiv. intros c1 c2 H st st'.
+  rewrite H. reflexivity. Qed.
+
+Lemma trans_cequiv : forall (c1 c2 c3 : com), cequiv c1 c2 -> cequiv c2 c3 -> cequiv c1 c3.
+Proof.
+  unfold cequiv. intros c1 c2 c3 H12 H23 st st'.
+  rewrite H12. apply H23. Qed.
+
+
+
+Theorem CAsgn_congruence : forall x a a',
+  aequiv a a' -> cequiv <{x := a}> <{x := a'}>.
+Proof.
+  intros x a a' Heqv st st'.
+  split; intros Hceval.
+  - (* -> *)
+    inversion Hceval. subst. apply E_Asgn.
+    rewrite Heqv. reflexivity.
+  - (* <- *)
+    inversion Hceval. subst. apply E_Asgn.
+    rewrite Heqv. reflexivity. Qed.
+
+Theorem CWhile_congruence : forall b b' c c',
+  bequiv b b' -> cequiv c c' ->
+  cequiv <{ while b do c end }> <{ while b' do c' end }>.
+Proof.
+  assert (A: forall (b b' : bexp) (c c' : com) (st st' : state),
+             bequiv b b' -> cequiv c c' ->
+             st =[ while b do c end ]=> st' -> st =[ while b' do c' end ]=> st').
+  { unfold bequiv, cequiv.
+    intros b b' c c' st st' Hbe Hc1e Hce.
+    remember <{ while b do c end }> as cwhile eqn:Heqcwhile.
+    induction Hce; inversion Heqcwhile; subst.
+    + (* E_WhileFalse *)
+      apply E_WhileFalse. rewrite <- Hbe. apply H.
+    + (* E_WhileTrue *)
+      apply E_WhileTrue with (st' := st').
+      * (* show loop runs *) rewrite <- Hbe. apply H.
+      * (* body execution *)
+        apply (Hc1e st st'). apply Hce1.
+      * (* subsequent loop execution *)
+        apply IHHce2. reflexivity.
+  }
+  intros. split.
+  - apply A; assumption.
+  - apply A.
+    + apply sym_bequiv. assumption.
+    + apply sym_cequiv. assumption.
+Qed.
+
+Theorem CSeq_congruence : forall c1 c1' c2 c2',
+  cequiv c1 c1' -> cequiv c2 c2' ->
+  cequiv <{ c1;c2 }> <{ c1';c2' }>.
+Proof.
+  unfold cequiv. intros c1 c1' c2 c2' Hec1 Hec2 st st'. 
+  split; intro H.
+  - inversion H. subst.
+    rewrite Hec1 in H2.
+    rewrite Hec2 in H5.
+    apply (E_Seq c1' c2' st st'0 st' H2 H5).
+  - inversion H. subst.
+    rewrite <- Hec1 in H2.
+    rewrite <- Hec2 in H5.
+    apply (E_Seq c1 c2 st st'0 st' H2 H5). Qed.
+
+Theorem CIf_congruence : forall b b' c1 c1' c2 c2',
+  bequiv b b' -> cequiv c1 c1' -> cequiv c2 c2' ->
+  cequiv <{ if b then c1 else c2 end }> <{ if b' then c1' else c2' end }>.
+Proof.
+  unfold bequiv, cequiv. intros b b' c1 c1' c2 c2' Heb Hec1 Hec2 st st'. 
+  split; intro H.
+  - inversion H.
+    + (* if true *)
+      subst. 
+      apply (E_IfTrue st st' b' c1' c2').
+      * rewrite <- Heb. assumption.
+      * rewrite <- Hec1. assumption.
+    + (* if false *)
+      subst. 
+      apply (E_IfFalse st st' b' c1' c2').
+      * rewrite <- Heb. assumption.
+      * rewrite <- Hec2. assumption.
+  - inversion H.
+    + (* if true *)
+      subst. 
+      apply (E_IfTrue st st' b c1 c2).
+      * rewrite Heb. assumption.
+      * rewrite Hec1. assumption.
+    + (* if false *)
+      subst. 
+      apply (E_IfFalse st st' b c1 c2).
+      * rewrite Heb. assumption.
+      * rewrite Hec2. assumption. Qed.
+
+
+
+Example congruence_example:
+  cequiv
+    (* Program 1: *)
+    <{ X := 0;
+       if (X = 0)
+       then
+         Y := 0
+       else
+         Y := 42
+       end }>
+    (* Program 2: *)
+    <{ X := 0;
+       if (X = 0)
+       then
+         Y := X - X (* <--- Changed here *)
+       else
+         Y := 42
+       end }>.
+Proof.
+  apply CSeq_congruence.
+  - apply refl_cequiv.
+  - apply CIf_congruence.
+    + apply refl_bequiv.
+    + apply CAsgn_congruence. unfold aequiv. simpl.
+      symmetry. apply minus_diag.
+    + apply refl_cequiv.
+Qed.
+
+
+
+
+Definition atrans_sound (atrans : aexp -> aexp) : Prop := forall (a : aexp), aequiv a (atrans a).
+Definition btrans_sound (btrans : bexp -> bexp) : Prop := forall (b : bexp), bequiv b (btrans b).
+Definition ctrans_sound (ctrans : com -> com  ) : Prop := forall (c : com), cequiv c (ctrans c).
+
+
+Fixpoint fold_constants_aexp (a : aexp) : aexp :=
+  match a with
+  | ANum n  => ANum n
+  | AId x   => AId x
+  | <{ a1 + a2 }> =>
+    match (fold_constants_aexp a1, fold_constants_aexp a2) with
+    | (ANum n1, ANum n2) => ANum (n1 + n2)
+    | (a1', a2') => <{ a1' + a2' }>
+    end
+  | <{ a1 - a2 }> =>
+    match (fold_constants_aexp a1, fold_constants_aexp a2) with
+    | (ANum n1, ANum n2) => ANum (n1 - n2)
+    | (a1', a2') => <{ a1' - a2' }>
+    end
+  | <{ a1 * a2 }> =>
+    match (fold_constants_aexp a1, fold_constants_aexp a2) with
+    | (ANum n1, ANum n2) => ANum (n1 * n2)
+    | (a1', a2') => <{ a1' * a2' }>
+    end
+  end.
+
+Example fold_aexp_ex1 : fold_constants_aexp <{ (1 + 2) * X }> = <{ 3 * X }>.
+Proof. reflexivity. Qed.
+
+Fixpoint fold_constants_bexp (b : bexp) : bexp :=
+  match b with
+  | <{true}>  => <{true}>
+  | <{false}> => <{false}>
+  | <{ a1 = a2 }> =>
+      match (fold_constants_aexp a1, fold_constants_aexp a2) with
+      | (ANum n1, ANum n2) => if n1 =? n2 then <{true}> else <{false}>
+      | (a1', a2')         => <{ a1' = a2' }>
+      end
+  | <{ a1 <= a2 }> =>
+      match (fold_constants_aexp a1, fold_constants_aexp a2) with
+      | (ANum n1, ANum n2) => if n1 <=? n2 then <{true}> else <{false}>
+      | (a1', a2')         => <{ a1' <= a2' }>
+      end
+  | <{ ~b1 }> =>
+      match (fold_constants_bexp b1) with
+      | <{true}>  => <{false}>
+      | <{false}> => <{true}>
+      | b1'       =><{ ~b1' }>
+      end
+  | <{ b1 && b2 }> =>
+      match (fold_constants_bexp b1, fold_constants_bexp b2) with
+      | (<{true}>, <{true}>)    => <{true}>
+      | (<{true}>, <{false}>)   => <{false}>
+      | (<{false}>, <{true}>)   => <{false}>
+      | (<{false}>, <{false}>)  => <{false}>
+      | (b1', b2')              => <{ b1' && b2' }>
+      end
+  end.
+
+Example fold_bexp_ex2 : fold_constants_bexp <{ (X = Y) && (0 = (2 - (1 + 1))) }> = <{ (X = Y) && true }>.
+Proof. reflexivity. Qed.
+
+Fixpoint fold_constants_com (c : com) : com :=
+  match c with
+  | <{ skip }>    => <{ skip }>
+  | <{ x := a }>  => <{ x := (fold_constants_aexp a) }>
+  | <{ c1 ; c2 }> => <{ fold_constants_com c1 ; fold_constants_com c2 }>
+  | <{ if b then c1 else c2 end }> =>
+      match fold_constants_bexp b with
+      | <{true}>  => fold_constants_com c1
+      | <{false}> => fold_constants_com c2
+      | b'        => <{ if b' then fold_constants_com c1 else fold_constants_com c2 end}>
+      end
+  | <{ while b do c1 end }> =>
+      match fold_constants_bexp b with
+      | <{true}>  => <{ while true do skip end }>
+      | <{false}> => <{ skip }>
+      | b'        => <{ while b' do (fold_constants_com c1) end }>
+      end
+  end.
+
+
+Theorem fold_constants_aexp_sound : atrans_sound fold_constants_aexp.
+Proof.
+  unfold atrans_sound. intros a. unfold aequiv. intros st.
+  induction a; simpl;
+    (* ANum and AId follow immediately *)
+    try reflexivity;
+    (* APlus, AMinus, and AMult follow from the IH
+       and the observation that
+              aeval st (<{ a1 + a2 }>)
+            = ANum ((aeval st a1) + (aeval st a2))
+            = aeval st (ANum ((aeval st a1) + (aeval st a2)))
+       (and similarly for AMinus/minus and AMult/mult) *)
+    try (destruct (fold_constants_aexp a1);
+         destruct (fold_constants_aexp a2);
+         rewrite IHa1; rewrite IHa2; reflexivity). Qed.
+
+Theorem fold_constants_bexp_sound: btrans_sound fold_constants_bexp.
+Proof.
+  unfold btrans_sound. intros b. unfold bequiv. intros st.
+  induction b;
+    (* true and false are immediate *)
+    try reflexivity.
+  - (* BEq *)
+    simpl.
+    remember (fold_constants_aexp a1) as a1' eqn:Heqa1'.
+    remember (fold_constants_aexp a2) as a2' eqn:Heqa2'.
+    replace (aeval st a1) with (aeval st a1') by
+       (subst a1'; rewrite <- fold_constants_aexp_sound; reflexivity).
+    replace (aeval st a2) with (aeval st a2') by
+       (subst a2'; rewrite <- fold_constants_aexp_sound; reflexivity).
+    destruct a1'; destruct a2'; try reflexivity.
+    (* The only interesting case is when both a1 and a2
+       become constants after folding *)
+      simpl. destruct (n =? n0); reflexivity.
+  - (* BLe *)
+    simpl.
+    remember (fold_constants_aexp a1) as a1' eqn:Heqa1'.
+    remember (fold_constants_aexp a2) as a2' eqn:Heqa2'.
+    assert (G1: aequiv a1 a1'). { subst a1'. apply (fold_constants_aexp_sound a1). }
+    replace (aeval st a1) with (aeval st a1') by (rewrite G1; reflexivity).
+    assert (G2: aequiv a2 a2'). { subst a2'. apply (fold_constants_aexp_sound a2). }
+    replace (aeval st a2) with (aeval st a2') by (rewrite G2; reflexivity).
+    destruct a1'; destruct a2'; try reflexivity.
+    simpl. destruct (n <=? n0); reflexivity.
+  - (* BNot *)
+    simpl. remember (fold_constants_bexp b) as b' eqn:Heqb'.
+    rewrite IHb.
+    destruct b'; reflexivity.
+  - (* BAnd *)
+    simpl.
+    remember (fold_constants_bexp b1) as b1' eqn:Heqb1'.
+    remember (fold_constants_bexp b2) as b2' eqn:Heqb2'.
+    rewrite IHb1. rewrite IHb2.
+    destruct b1'; destruct b2'; reflexivity.
+Qed.
+
+Theorem fold_constants_com_sound : ctrans_sound fold_constants_com.
+Proof.
+  unfold ctrans_sound. intros c.
+  induction c; simpl.
+  - (* skip *) apply refl_cequiv.
+  - (* := *) apply CAsgn_congruence.
+             apply fold_constants_aexp_sound.
+  - (* ; *)  apply CSeq_congruence; assumption.
+  - (* if *)
+    assert (bequiv b (fold_constants_bexp b)). { apply fold_constants_bexp_sound. }
+    destruct (fold_constants_bexp b) eqn:Heqb;
+      try (apply CIf_congruence; assumption).
+      (* (If the optimization doesn't eliminate the if, then the
+          result is easy to prove from the IH and
+          fold_constants_bexp_sound.) *)
+    + (* b always true *)
+      apply trans_cequiv with c1; try assumption.
+      apply if_true; assumption.
+    + (* b always false *)
+      apply trans_cequiv with c2; try assumption.
+      apply if_false; assumption.
+  - (* while *)
+    destruct (fold_constants_bexp b) eqn:Heqb.
+    + (* while true  *)  apply while_true.  rewrite <- Heqb. apply fold_constants_bexp_sound.
+    + (* while false *)  apply while_false. rewrite <- Heqb. apply fold_constants_bexp_sound.
+    + (* while a = b *)  apply CWhile_congruence. rewrite <- Heqb. apply fold_constants_bexp_sound. apply IHc.
+    + (* while a <= b *) apply CWhile_congruence. rewrite <- Heqb. apply fold_constants_bexp_sound. apply IHc.
+    + (* while ~f *)     apply CWhile_congruence. rewrite <- Heqb. apply fold_constants_bexp_sound. apply IHc.
+    + (* while p && f *) apply CWhile_congruence. rewrite <- Heqb. apply fold_constants_bexp_sound. apply IHc.
+Qed.
+
+
+
+Fixpoint optimize_0plus_aexp (a : aexp) : aexp :=
+  match a with
+  | ANum n  => ANum n
+  | AId x   => AId x
+  | <{ 0 + a2 }> => optimize_0plus_aexp a2
+  | <{ a1 + a2 }> =>
+    match (optimize_0plus_aexp a1, optimize_0plus_aexp a2) with
+    | (a1', a2') => <{ a1' + a2' }>
+    end
+  | <{ a1 - a2 }> =>
+    match (optimize_0plus_aexp a1, optimize_0plus_aexp a2) with
+    | (a1', a2') => <{ a1' - a2' }>
+    end
+  | <{ a1 * a2 }> =>
+    match (optimize_0plus_aexp a1, optimize_0plus_aexp a2) with
+    | (a1', a2') => <{ a1' * a2' }>
+    end
+  end.
+
+Fixpoint optimize_0plus_bexp (b : bexp) : bexp :=
+  match b with
+  | <{true}>  => <{true}>
+  | <{false}> => <{false}>
+  | <{ a1 = a2 }> =>
+      match (optimize_0plus_aexp a1, optimize_0plus_aexp a2) with
+      | (a1', a2')         => <{ a1' = a2' }>
+      end
+  | <{ a1 <= a2 }> =>
+      match (optimize_0plus_aexp a1, optimize_0plus_aexp a2) with
+      | (a1', a2')         => <{ a1' <= a2' }>
+      end
+  | <{ ~b1 }> =>
+      match (optimize_0plus_bexp b1) with
+      | b1'       =><{ ~b1' }>
+      end
+  | <{ b1 && b2 }> =>
+      match (optimize_0plus_bexp b1, optimize_0plus_bexp b2) with
+      | (b1', b2')              => <{ b1' && b2' }>
+      end
+  end.
+
+Fixpoint optimize_0plus_com (c : com) : com :=
+  match c with
+  | <{ skip }>    => <{ skip }>
+  | <{ x := a }>  => <{ x := (optimize_0plus_aexp a) }>
+  | <{ c1 ; c2 }> => <{ optimize_0plus_com c1 ; optimize_0plus_com c2 }>
+  | <{ if b then c1 else c2 end }> => <{ if optimize_0plus_bexp b then optimize_0plus_com c1 else optimize_0plus_com c2 end}>
+  | <{ while b do c1 end }> => <{ while optimize_0plus_bexp b do (optimize_0plus_com c1) end }>
+  end.
+
+Example optimize_0plus_aexp_ex: optimize_0plus_aexp <{ 0 + X }> = <{ X }>.
+Proof. reflexivity. Qed.
+
+Example optimize_0plus_com_ex: 
+  optimize_0plus_com <{ if (0 + X <= Y) then X := 0 + Y; Y := 0 + X else Y := 0 + 1 end }> =
+  <{ if (X <= Y) then X := Y; Y := X else Y := 1 end }>.
+Proof. reflexivity. Qed.
+
+Theorem optimize_0plus_aexp_sound : atrans_sound optimize_0plus_aexp.
+Proof.
+  unfold atrans_sound. intro a. unfold aequiv. intros st.
+  induction a; simpl.
+  - (* n *) reflexivity.
+  - (* X *) reflexivity.
+  - (* + *) 
+    rewrite IHa1. rewrite IHa2.
+    destruct a1 eqn:Ea1; try (reflexivity). (* match aexp, trivial for all except Nums *)
+    destruct n eqn:En; simpl; reflexivity. (* match specific num *)
+  - (* - *)
+    rewrite IHa1. rewrite IHa2. reflexivity.
+  - (* * *)
+    rewrite IHa1. rewrite IHa2. reflexivity.
+Qed.
+
+Theorem optimize_0plus_bexp_sound: btrans_sound optimize_0plus_bexp.
+Proof.
+  unfold btrans_sound. intro b. unfold bequiv. intros st.
+  induction b; simpl; 
+    try (reflexivity);
+    try ( rewrite (optimize_0plus_aexp_sound a1);
+          rewrite (optimize_0plus_aexp_sound a2);
+          reflexivity).
+    try (rewrite IHb; reflexivity).
+  - (* && *)
+    rewrite IHb1.
+    rewrite IHb2.
+    reflexivity.
+Qed.
+
+Theorem optimize_0plus_com_sound : ctrans_sound optimize_0plus_com.
+Proof.
+  unfold ctrans_sound. intro c. 
+  induction c; unfold cequiv; intros st st'; simpl.
+  - (* skip *) apply refl_cequiv.
+  - (* :=   *) apply CAsgn_congruence. apply optimize_0plus_aexp_sound.
+  - (* ;    *) apply CSeq_congruence.  apply IHc1. apply IHc2.
+  - (* if   *) apply CIf_congruence. apply optimize_0plus_bexp_sound. apply IHc1. apply IHc2.
+  - (* whle *) apply CWhile_congruence. apply optimize_0plus_bexp_sound. apply IHc.
+Qed.
